ITree/EffectAlgebra.lean
@@ -1,7 +1,7 @@
 import ITree.Monad
 
-abbrev naturalTransformation (ε1 : Type u → Type v1) (ε2 : Type u → Type v2) :=
-  ∀ {α : Type u}, ε1 α → ε2 α
+abbrev naturalTransformation (ε1 : Type u → Type v1) (ε2 : Type (max u v) → Type v2) :=
+  ∀ {α : Type u}, ε1 α → ε2 (ULift α)
 infixr:50 " ⟶ "=> naturalTransformation
 
 inductive SumE (ε1 ε2 : Type u → Type v) : Type u → Type v
@@ -27,8 +27,8 @@ inductive IterState (ι : Type u) (ρ : Type v)
   | done  (r : ρ)
   | recur (i : ι)
 
-class MonadIter (m : Type u -> Type v) where
-  iter : {ρ ι : Type u} → (ι -> m (IterState ι ρ)) -> ι -> m ρ
+class MonadIter (m : Type max i r → Type v) where
+  iter {ρ : Type r} {ι : Type i} : (ι → m (IterState ι ρ)) → ι → m (ULift ρ)
 
 namespace ITree
 
@@ -36,14 +36,15 @@ inductive IterMode {ε ρ ι}
   | iterS (i : ι)
   | bindS (t : ITree ε (IterState ι ρ))
 
-def iter {ε ρ ι} (step : ι → ITree ε (IterState ι ρ)) (i : ι) : ITree ε ρ :=
+def iter {ε : Type u → Type v} {ρ : Type r} {ι : Type i}
+  (step : ι → ITree ε (IterState ι ρ)) (i : ι) : ITree ε (ULift ρ) :=
   .corec' (fun rec (s : IterMode) =>
     match s with
     | .bindS t =>
       match t.dest with
       | ⟨.ret v, _⟩ =>
         match v with
-        | .done r => .inl <| ret r
+        | .done r => .inl <| ret <| .up r
         | .recur l => .inr <| tau' <| rec <| .bindS (step l)
       | ⟨.tau, c⟩ => .inr <| tau' <| rec <| .bindS <| c 0
       | ⟨.vis _ e, k⟩ => .inr <| vis' e <| fun a => rec <| .bindS <| k a
@@ -53,13 +54,17 @@ def iter {ε ρ ι} (step : ι → ITree ε (IterState ι ρ)) (i : ι) : ITree 
 instance {ε : Type u → Type v} : MonadIter (ITree ε) where
   iter := ITree.iter
 
-def interp {ε m : Type u → Type v} {ρ : Type u} [MonadIter m]
-  (handler : ε ⟶ m) (t : ITree ε ρ) : m ρ :=
-  MonadIter.iter (fun t =>
+def interp {ε : Type u → Type v}
+  [Monad m] [MonadIter.{r, max (max (max (u + 1) r) v) u, _} m]
+  (h : ∀ {α}, ε α → m (ULift.{max (max (u + 1) r) v, u} α))
+  : ∀ {ρ : Type r}, ITree ε ρ → m (ULift.{max (max (u + 1) r) v, r} ρ) :=
+  fun t =>
+  MonadIter.iter.{r, max (max (max (u + 1) r) v) u, _} (fun t =>
     match t.dest with
-    | ⟨.ret v, _⟩ => ret <| .done v
-    | ⟨.tau, c⟩ => ret <| .recur (c 0)
-    | ⟨.vis _ e, k⟩ => (handler e).bind <| fun a => ret <| .recur <| k a -- using >>= messes up universes
+    | ⟨.ret v, _⟩ => pure <| .done v
+    | ⟨.tau, c⟩ => pure <| .recur <| c 0
+    | ⟨.vis α e, k⟩ =>
+      Functor.map (fun a : ULift.{max (max (u + 1) r) v, _} α => .recur <| k a.down) (h e)
   ) t
 
 end ITree
